\begin{frame}[fragile]
\frametitle{The Expression Problem}
\begin{block}{Another example}
\begin{lstlisting}[style=haskell,mathescape]
data Either a b = Left a | Right b

leftor :: a -> Either a b -> a
leftor _ (Left a) = a
leftor a (Right _) = a
\end{lstlisting}
\end{block}
\end{frame}

\begin{frame}[fragile]
\frametitle{The Expression Problem}
\begin{block}{Add \lstinline[style=haskell]{None} case}
\begin{lstlisting}[style=haskell,mathescape]
data Either a b = Left a | Right b | None

leftor :: a -> Either a b -> a
leftor _ (Left a)  = a
leftor a (Right _) = a
leftor a None      = a
\end{lstlisting}
\end{block}
\end{frame}

\begin{frame}[fragile]
\frametitle{The Expression Problem}
\begin{block}{Another example}
We'd like to write \lstinline[style=haskell]{leftor} once, and for both data types.
\end{block}
\end{frame}

\begin{frame}[fragile]
\frametitle{The Expression Problem}
\begin{block}{\lstinline[style=haskell]{Both} case}
\begin{lstlisting}[style=haskell,mathescape]
data Either a b = Left a | Right b
data Prolly a b = This a | That  b | None 

leftor :: Leftish p => a -> t a b -> a
leftor = $\ldots$
\end{lstlisting}
\end{block}
\end{frame}

\begin{frame}[fragile]
\frametitle{The Expression Problem}
\begin{block}{Leftish}
We want to abstract
\begin{itemize}
\item the \textbf{view} of \lstinline{(a)}
\item \textbf{possibly existing} in \lstinline{(t a b)}
\end{itemize}
\end{block}
\end{frame}

\begin{frame}[fragile]
\frametitle{The Expression Problem}
\begin{block}{Leftish \textbf{view}}
\begin{lstlisting}[style=haskell,mathescape]
type LeftishView t a b =
  (a `->` `Identity` a) -> (t a b `->` `Identity` (t a b))
\end{lstlisting}
\end{block}
\begin{itemize}
\item<1-> \lstinline[style=haskell]{Identity}
\item<2-> \lstinline[style=haskell]{(->)}
\end{itemize}
\end{frame}

\begin{frame}[fragile]
\frametitle{The Expression Problem}
\begin{block}{Leftish \textbf{view}}
\begin{lstlisting}[style=haskell,mathescape]
type LeftishView p f t a b =
  (a $`p`$ f a) -> (t a b $`p`$ f (t a b))
\end{lstlisting}
\end{block}
\end{frame}

\begin{frame}[fragile]
\frametitle{The Expression Problem}
\begin{block}{Left \textbf{prism}}
\begin{lstlisting}[style=haskell,mathescape]
type LeftPrism p f t a b =
  (Choice p, Applicative f) => 
    (a $`p`$ f a) -> (t a b $`p`$ f (t a b))
\end{lstlisting}
\end{block}
\end{frame}

\begin{frame}[fragile]
\frametitle{The Expression Problem}
\begin{block}{Leftish type-class}
\begin{lstlisting}[style=haskell,mathescape]
class Leftish p f t where
  _Leftish ::
    (a $`p`$ f a) -> (t a b $`p`$ f (t a b))

instance (Choice p, Applicative f) =>
  Leftish p f Either where
instance (Choice p, Applicative f) =>
  Leftish p f Prolly where
\end{lstlisting}
\end{block}
\end{frame}

\begin{frame}[fragile]
\frametitle{The Expression Problem}
\begin{block}{\lstinline{leftor} from Leftish type-class}
\begin{lstlisting}[style=haskell,mathescape]
leftor ::
  LeftLike (->) (Const (First a)) t =>
  a
  -> t a b
  -> a 
leftor a x =
  fromMaybe a (x ^? _Leftish)
\end{lstlisting}
\end{block}
\end{frame}

\begin{frame}[fragile]
\frametitle{The Expression Problem}
\begin{block}{\lstinline{leftor} from Leftish type-class}
\begin{lstlisting}[style=haskell,mathescape]
leftor ::
  LeftLike (->) (Const (First a)) t =>
  a
  -> t a b
  -> a 
leftor a x =
  fromMaybe a (x ^? _Leftish)
\end{lstlisting}
\end{block}
\end{frame}
